real and uint case

SmartContracts/ModellingOfBugs/DeusFinacePriceOracleManipulation/ErrorneousAccounting.dfy
@@ -24,27 +24,27 @@ import opened NonNativeTypes
 
 class errorneous
 {
-  var amount0Out : real, reserve0 : real, reserve1 : real;
-  var token0 : map<errorneous, real>, token1 : map<errorneous, real>;
+  var amount0Out : nat, reserve0 : nat, reserve1 : nat;
+  var token0 : map<errorneous, nat>, token1 : map<errorneous, nat>;
 
-  method swap(amount1Out : real, to : errorneous)
+  method swap(amount1Out : nat, to : errorneous)
     requires this in token0 && this in token1
     requires token1[this] == reserve1
-    requires reserve0 - amount0Out == token0[this] && reserve0 > amount0Out >= 0.0
-    requires amount0Out > 0.0 && reserve1 > 0.0 && reserve0 > 0.0
+    requires reserve0 - amount0Out == token0[this] && reserve0 > amount0Out >= 0
+    requires amount0Out > 0 && reserve1 > 0 && reserve0 > 0
 
     modifies this
 
     ensures reserve0 * reserve1 >= old(reserve0) * old(reserve1)
   {
-    if(0.0 < amount1Out < token1[this])
+    if(0 < amount1Out < token1[this])
     {
       token1 := token1[this := token1[this] - amount1Out];
       token0 := token0[this := havoc()];
       var balance0, balance1 := token0[this], token1[this];
-      var amount0in : real := balance0 - (reserve0 - amount0Out);
-      var balance0Adj : real := balance0 * 10000.0 - amount0in * 22.0;
-      if(balance0Adj * balance1 >= reserve0 * reserve1 * 1000.0)
+      var amount0in : int := balance0 - (reserve0 - amount0Out);
+      var balance0Adj : nat := balance0 * 10000 - amount0in * 22;
+      if(balance0Adj * balance1 >= reserve0 * reserve1 * 1000)
       {
         reserve0, reserve1 := balance0, balance1;
       }
@@ -52,5 +52,38 @@ class errorneous
   }
 }
 
-function method {:extern} havoc() : real
-  ensures havoc() > 0.0
+function method {:extern} havoc() : nat
+  ensures havoc() > 0
+
+// class errorneous
+// {
+//   var amount0Out : real, reserve0 : real, reserve1 : real;
+//   var token0 : map<errorneous, real>, token1 : map<errorneous, real>;
+
+//   method swap(amount1Out : real, to : errorneous)
+//     requires this in token0 && this in token1
+//     requires token1[this] == reserve1
+//     requires reserve0 - amount0Out == token0[this] && reserve0 > amount0Out >= 0.0
+//     requires amount0Out > 0.0 && reserve1 > 0.0 && reserve0 > 0.0
+
+//     modifies this
+
+//     ensures reserve0 * reserve1 >= old(reserve0) * old(reserve1)
+//   {
+//     if(0.0 < amount1Out < token1[this])
+//     {
+//       token1 := token1[this := token1[this] - amount1Out];
+//       token0 := token0[this := havoc()];
+//       var balance0, balance1 := token0[this], token1[this];
+//       var amount0in : real := balance0 - (reserve0 - amount0Out);
+//       var balance0Adj : real := balance0 * 10000.0 - amount0in * 22.0;
+//       if(balance0Adj * balance1 >= reserve0 * reserve1 * 1000.0)
+//       {
+//         reserve0, reserve1 := balance0, balance1;
+//       }
+//     }
+//   }
+// }
+
+// function method {:extern} havoc() : real
+//   ensures havoc() > 0.0
